sail-riscv/memcpy.v
@@ -93,14 +93,14 @@ Proof.
   unfold translateAddr. red_sim. rewrite mstatus_nextPC cur_privilege_nextPC.
   apply sim_effectivePrivilege; [done|]. red_sim.
   unfold translateAddr_priv. red_sim.
-  apply: sim_read_reg_l; [done|]. red_sim.
-  apply: sim_read_reg_l; [done|]. red_sim.
+  apply: sim_read_reg_l; [solve_of_regval_regval_of|]. red_sim.
+  apply: sim_read_reg_l; [solve_of_regval_regval_of|]. red_sim.
   unfold translationMode.
   have -> : (cur_privilege regs) = Machine by destruct (cur_privilege regs). red_sim.
-  apply: sim_read_reg_l; [done|]. red_sim. rewrite x11_nextPC.
+  apply: sim_read_reg_l; [solve_of_regval_regval_of|]. red_sim. rewrite x11_nextPC.
   unfold mem_read. red_sim.
-  apply: sim_read_reg_l; [done|]. red_sim.
-  apply: sim_read_reg_l; [done|]. red_sim. rewrite mstatus_nextPC.
+  apply: sim_read_reg_l; [solve_of_regval_regval_of|]. red_sim.
+  apply: sim_read_reg_l; [solve_of_regval_regval_of|]. red_sim. rewrite mstatus_nextPC.
   apply sim_effectivePrivilege; [done|]. red_sim.
   rewrite Hassume. red_sim.
   rewrite if_false; [|shelve]. rewrite if_true; [|shelve]. red_sim.
@@ -116,7 +116,7 @@ Proof.
     + rewrite ->Hassume1, Hassume2, !bv_add_unsigned, !bv_unsigned_BV in *.
       unfold bv_wrap, bv_modulus in *. lia.
   - by rewrite mword_to_bv_add_vec.
-  - rewrite mword_to_bv_EXTS // mword_to_bv_to_mword //.
+  - rewrite mword_to_bv_sign_extend' // mword_to_bv_to_mword //.
   - rewrite mword_to_bv_add_vec //.
     Unshelve. all: exact: inhabitant.
 Qed.
@@ -130,14 +130,14 @@ Proof.
   unfold translateAddr. red_sim. rewrite mstatus_nextPC cur_privilege_nextPC.
   apply sim_effectivePrivilege; [done|]. red_sim.
   unfold translateAddr_priv. red_sim.
-  apply: sim_read_reg_l; [done|]. red_sim.
-  apply: sim_read_reg_l; [done|]. red_sim.
+  apply: sim_read_reg_l; [solve_of_regval_regval_of|]. red_sim.
+  apply: sim_read_reg_l; [solve_of_regval_regval_of|]. red_sim.
   unfold translationMode.
   have -> : (cur_privilege regs) = Machine by destruct (cur_privilege regs). red_sim.
-  apply: sim_read_reg_l; [done|]. red_sim. rewrite x10_nextPC.
+  apply: sim_read_reg_l; [solve_of_regval_regval_of|]. red_sim. rewrite x10_nextPC.
   unfold mem_write_value, mem_write_value_meta. red_sim.
-  apply: sim_read_reg_l; [done|]. red_sim.
-  apply: sim_read_reg_l; [done|]. red_sim. rewrite mstatus_nextPC cur_privilege_nextPC.
+  apply: sim_read_reg_l; [solve_of_regval_regval_of|]. red_sim.
+  apply: sim_read_reg_l; [solve_of_regval_regval_of|]. red_sim. rewrite mstatus_nextPC cur_privilege_nextPC.
   apply sim_effectivePrivilege; [done|]. red_sim.
   rewrite Hassume. red_sim.
   rewrite if_false; [|shelve]. rewrite if_true; [|shelve]. red_sim.
@@ -195,7 +195,7 @@ Proof.
   move => regs. unfold step_cpu, a18.
   red_sim. unfold execute. red_sim. unfold execute_BTYPE.
   red_sim.
-  apply: sim_read_reg_l; [done|]. red_sim. rewrite x12_nextPC.
+  apply: sim_read_reg_l; [solve_of_regval_regval_of|]. red_sim. rewrite x12_nextPC.
   destruct (neq_vec (x12 regs) zero_reg) eqn: Hx12; unfold neq_vec in Hx12; sim_simpl_hyp Hx12; red_sim.
   - apply: (sim_tcases 0); [done|]. red_sim.
     rewrite bit_to_bool_false; [|shelve]. red_sim.
